More thoughts about assign_thm

compiler/backend/bvp_to_wordScript.sml
@@ -26,6 +26,9 @@ val assign_def = Define `
         then (Assign (adjust_var dest) (Const (0w - n2w (Num (4 * (0 - i))))),l)
         else (Assign (adjust_var dest) (Const (n2w (Num (4 * i)))),l)
     | GlobalsPtr => (Assign (adjust_var dest) (Lookup Globals),l)
+    | SetGlobalsPtr => (Seq (Set Globals (Var (adjust_var (HD args))))
+                            (Assign (adjust_var dest) (Const 0w (* TODO: Unit *))),l)
+    | El => (Assign (adjust_var dest) (Load (Op Add (MAP (Var o adjust_var) args))),l)
     | _ => (Skip:'a wordLang$prog,l)`;
 
 val comp_def = Define `
